Strip lemmas from the semaphore proof for the barrier

formal-proofs/theories/lib/interruptible_semaphore/interruptible_semaphore.v
@@ -41,6 +41,7 @@ From iris.program_logic Require Import atomic.
 Require Import SegmentQueue.lib.infinite_array.infinite_array_impl.
 Require Import SegmentQueue.lib.infinite_array.iterator.
 Require Import SegmentQueue.lib.util.interruptibly.
+Require Import SegmentQueue.lib.thread_queue.thread_queue_as_counter.
 
 Section proof.
 
@@ -61,11 +62,9 @@ Variable (segment_size: positive).
 
 Definition is_semaphore_inv (R : iProp) (γ: gname) (availablePermits: nat) (p: loc)
   (epℓ eℓ dpℓ dℓ: loc) (γa γtq γe γd: gname) :=
-  (∃ l deqFront,
-  ([∗ list] _ ∈ seq 0 availablePermits, R) ∗
+  (∃ v, ([∗ list] _ ∈ seq 0 availablePermits, R) ∗
    own γ (● (Excl' availablePermits)) ∗
-   is_thread_queue (N .@ "tq") Nth segment_size True R γa γtq γe γd eℓ epℓ dℓ dpℓ l deqFront ∗
-   let v := count_matching still_present (drop deqFront l) in
+   thread_queue_as_counter (N .@ "tq") Nth segment_size True R γa γtq γe γd eℓ epℓ dℓ dpℓ v ∗
    p ↦ #(availablePermits - v) ∗ ⌜(availablePermits = 0 ∨ v = 0)%nat⌝)%I.
 
 Definition is_semaphore (R : iProp) (γ: gname) (p: loc)
@@ -75,14 +74,6 @@ Definition is_semaphore (R : iProp) (γ: gname) (p: loc)
 
 Definition semaphore_permits γ availablePermits :=
   own γ (◯ (Excl' availablePermits)).
-
-Theorem count_matching_find_index_Some A (P: A -> Prop) (H': forall x, Decision (P x)) l:
-  count_matching P l > 0 -> is_Some (find_index P l).
-Proof.
-  induction l; simpl; first done.
-  destruct (decide (P a)); first by eauto.
-  destruct (find_index P l); by eauto.
-Qed.
 
 Lemma new_semaphore_spec (n: nat) R:
   {{{ ([∗ list] x ∈ replicate n R, x) }}}
@@ -106,9 +97,13 @@ Proof.
           with "[-HΦ HFrag]") as "#HInv".
   {
     iExists _.
-    rewrite /is_semaphore_inv. iExists [], O.
-    iFrame. simpl. rewrite Z.sub_0_r. iFrame.
-    iSplitL; last by iPureIntro; right.
+    rewrite /is_semaphore_inv. iExists O. iFrame "HAuth".
+    rewrite Z.sub_0_r. iFrame "Hp".
+    iSplitL "HRs".
+    2: {
+      iSplitL; last by iPureIntro; right.
+      iExists _, _. by iFrame.
+    }
     iApply (big_sepL_forall' with "HRs").
     by rewrite replicate_length seq_length.
     intros ? ? ?. rewrite lookup_replicate. by intros _ [-> _].
@@ -128,52 +123,26 @@ Lemma resume_in_semaphore_spec R γ p epℓ eℓ dpℓ dℓ γa γtq γe γd:
   {{{ RET #(); True }}}.
 Proof.
   iIntros "#HSemInv #HPermInv" (Φ) "!> HAwak HΦ". wp_lam. wp_pures.
-  awp_apply (try_deque_thread_spec (N .@ "tq") with "HAwak") without "HΦ".
-  iInv "HSemInv" as (? ? deqFront') "(HPerms & >HAuth & HTq & HRest)".
+  awp_apply (try_deque_thread_as_counter_spec (N .@ "tq") with "HAwak") without "HΦ".
+  iInv "HSemInv" as (? ?) "(HPerms & >HAuth & HTq & HRest)".
   iAaccIntro with "HTq".
   {
     iIntros "HTq !>".
     iSplitL; last done.
-    iExists _, _, _. iFrame.
+    iExists _, _. iFrame.
   }
-  iIntros (?) "[_ HState]".
-  iDestruct "HState" as (i) "[HState|HState]".
+  iIntros (?) "(_ & HTq & HState)".
+  iDestruct "HState" as "[->|HState]".
   {
-    iDestruct "HState" as "[(HEl & -> & HTq) HRend]".
-    iDestruct "HEl" as %HEl.
-    iSplitL.
-    2: {
-      iIntros "!> HΦ".
-      wp_pures.
-      by iApply "HΦ".
-    }
-    destruct (decide (i < deqFront')%nat).
-    2: {
-      iDestruct "HTq" as "(_ & (_ & >HResumerStage & _) & _)".
-      rewrite big_sepL_forall.
-      iSpecialize ("HResumerStage" $! (i - deqFront')%nat _ with "[]").
-      {
-        iPureIntro.
-        rewrite lookup_drop.
-        replace (deqFront' + (i - deqFront'))%nat with i by lia.
-        rewrite list_lookup_alter.
-        rewrite HEl. done.
-      }
-      simpl.
-      iDestruct "HResumerStage" as %HContra.
-      discriminate.
-    }
-    iExists _, _, _. iFrame "HPerms HAuth HTq".
-    iDestruct "HRest" as "[Hp >%]".
-    rewrite drop_alter //.
-    iSplitL "Hp"; done.
+    iSplitL; first by iExists _, _; iFrame.
+    iIntros "!> HΦ". wp_pures. by iApply "HΦ".
   }
 
-  iDestruct "HState" as (? ?) "[#[HIsThread HThreadLocs] [HState|HState]]".
+  iDestruct "HState" as (? ? ?) "(-> & #[HIsThread HThreadLocs] &
+    [[HResTok #HRendRes]|HNoPerms])".
   2: {
-    iDestruct "HState" as "[HState (-> & HTq & HNoPerms)]".
     iSplitR "HNoPerms".
-    by iExists _, _, _; iFrame.
+    by iExists _, _; iFrame.
     iIntros "!> HΦ". wp_pures.
     awp_apply (unpark_spec with "HIsThread") without "HΦ".
     iAaccIntro with "HNoPerms".
@@ -181,99 +150,18 @@ Proof.
     iIntros "HPerms !> HΦ". wp_pures. by iApply "HΦ".
   }
   {
-    iDestruct "HState" as (HEl ?) "(HTq & #HRendRes & HResTok)".
-    iDestruct "HRest" as "[Hp >%]".
-    subst.
-    iSplitR "HResTok".
-    {
-      destruct (decide (i < deqFront')%nat).
-      2: {
-        iDestruct "HTq" as "(_ & (_ & >HResumerStage & _) & _)".
-        rewrite big_sepL_forall.
-        iSpecialize ("HResumerStage" $! (i - deqFront')%nat _ with "[]").
-        {
-          iPureIntro.
-          rewrite lookup_drop.
-          replace (deqFront' + (i - deqFront'))%nat with i by lia.
-          rewrite list_lookup_alter.
-          rewrite HEl. done.
-        }
-        simpl.
-        iDestruct "HResumerStage" as %HContra.
-
-        discriminate.
-      }
-      iExists _, _, _. iFrame "HTq HAuth".
-      rewrite drop_alter //.
-      by iFrame.
-    }
+    iSplitR "HResTok"; first by iExists _, _; iFrame.
     iIntros "!> HΦ". wp_pures.
-    awp_apply (unpark_spec with "HIsThread") without "HΦ".
 
-    iInv "HSemInv" as (? l' ?) "(HPerms & >HAuth & (HInfArr & HListContents & HRest') & HRest)".
-    iDestruct "HListContents" as "(HLi1 & HLi2 & >HTqAuth & HLi4 & HLi5 & HCellResources)".
-
-    iDestruct "HRendRes" as (? ?) "HRendRes".
-
-    iDestruct (cell_list_contents_done_agree with "HTqAuth HRendRes")
-              as %HEl'.
-
-    iDestruct (cell_list_contents_ra_locs with "HTqAuth HThreadLocs")
-              as %[? HEl''].
-    simplify_eq.
-
-    iDestruct (big_sepL_lookup_acc with "HCellResources") as "[HRes HRRsRestore]".
-    done.
-    simpl.
-    iAssert (resumer_token γtq i -∗ resumer_token γtq i -∗ False)%I as "HNoResTok".
-    {
-      iIntros "HResTok HResTok'".
-      iDestruct (own_valid_2 with "HResTok HResTok'") as %HH.
-      rewrite -auth_frag_op in HH. exfalso. move: HH.
-      rewrite auth_frag_valid pair_valid list_op_singletonM list_lookup_valid /=.
-      intros [_ HValid]. specialize (HValid i). move: HValid.
-      rewrite list_lookup_singletonM.
-      intros HValid.
-      destruct HValid as [[[_ []] _] _].
-    }
-    iDestruct "HRes" as (ℓ) "(HArrMapsto & HTH & HIsSus & HIsRes & HCancHandle &
-                             HConds)".
-    iDestruct "HConds" as "[[HInhTok [HNoPerms|>HResTok']]|
-                           [Hℓ [HR [[_ >HResTok']|HNoPerms]]]]";
-      try iDestruct ("HNoResTok" with "HResTok HResTok'") as %[].
-
-    all: iAaccIntro with "HNoPerms".
-    3: {
-      iFrame "HResTok".
-      iIntros ">HNoPerms !>". iExists _, _, _. iFrame.
-      iApply ("HRRsRestore" with "[-]").
-      iExists _. iFrame.
-      iRight; iFrame.
-    }
-    {
-      iFrame "HResTok".
-      iIntros ">HNoPerms !>". iExists _, _, _. iFrame.
-      iApply ("HRRsRestore" with "[-]").
-      iExists _. iFrame.
-    }
-
-    {
-      iIntros "HThPerms !>".
-      iSplitL.
-      2: iIntros "HΦ"; wp_pures; by iApply "HΦ".
-      iExists _, _, _. iFrame.
-      iApply ("HRRsRestore" with "[-]").
-      iExists _. iFrame. iLeft. iFrame.
-    }
-
-    {
-      iIntros "HThPerms !>".
-      iSplitL.
-      2: iIntros "HΦ"; wp_pures; by iApply "HΦ".
-      iExists _, _, _. iFrame.
-      iApply ("HRRsRestore" with "[-]").
-      iExists _. iFrame. iRight. iFrame. iLeft. iFrame.
-    }
+    awp_apply (thread_queue_as_counter_unpark_spec with
+                   "HRendRes HIsThread HThreadLocs") without "HΦ".
+    iInv "HSemInv" as (? ?) "(HPerms & >HAuth & HTq & HRest)".
+    iCombine "HResTok" "HTq" as "HAacc".
+    iAaccIntro with "HAacc".
+    { iIntros "[$ HTq]". iExists _, _. by iFrame. }
+    iIntros "HTq". iSplitL.
+    by iExists _, _; iFrame.
+    iIntros "!> HΦ". wp_pures. by iApply "HΦ".
   }
 Qed.
 
@@ -286,10 +174,9 @@ Theorem release_semaphore_spec R γ (p epℓ eℓ dpℓ dℓ: loc) γa γtq γe 
 Proof.
   iIntros "#HSemInv #HPermInv" (Φ) "!> HR HΦ". wp_lam. wp_pures.
   wp_bind (FAA _ _).
-  iInv "HSemInv" as (availablePermits' l deqFront)
+  iInv "HSemInv" as (availablePermits' v)
                       "(HPerms & >HAuth & HTq & Hp & >HPure)" "HInvClose".
   iDestruct "HPure" as %HPure.
-  remember (count_matching _ _) as v.
   remember (availablePermits' - v) as op.
   wp_faa.
   destruct (decide (0 <= op)).
@@ -303,11 +190,10 @@ Proof.
       apply (exclusive_local_update _ (Excl (1 + availablePermits)%nat)).
       done.
     }
-    repeat rewrite Nat.add_1_r.
     iMod ("HInvClose'" with "[HFrag]") as "_"; first by eauto.
     iMod ("HInvClose" with "[-HΦ]") as "_".
     {
-      iExists _, _, _. simpl. iFrame "HAuth HTq". simpl.
+      iExists _, _. simpl. iFrame "HAuth HTq". simpl.
       iFrame "HR".
       iSplitL "HPerms".
       {
@@ -317,7 +203,7 @@ Proof.
       }
       iSplitL.
       {
-        rewrite -Heqv Heqop.
+        rewrite Heqop.
         replace (S availablePermits - v) with (availablePermits - v + 1).
         done.
         lia.
@@ -329,50 +215,14 @@ Proof.
     destruct (decide (0 <= op)); try lia. wp_pures. by iApply "HΦ".
   }
 
-  assert (v > 0) as HExistsNondequed by lia.
-  move: HExistsNondequed. subst. move=> HExistsNondequed.
-
-  apply count_matching_find_index_Some in HExistsNondequed.
-  destruct HExistsNondequed as [? HFindIndex].
-
-  iDestruct "HTq" as "(HInfArr & HListContents & % & HRest)".
-  iDestruct (cell_list_contents_register_for_dequeue
-               with "HR HListContents") as ">[[HAwak #HDeqFront] [HListContents HCounts]]".
-  by eauto.
-  iDestruct "HCounts" as %HCounts.
+  iMod (thread_as_counter_register_for_dequeue with "HR HTq")
+    as "[HAwak HTq]"; first by lia.
 
   iMod ("HInvClose" with "[-HAwak HΦ]") as "_".
   {
-    iExists _, _, _. iFrame "HListContents". iFrame.
-    iSplitL "HRest".
-    {
-      iDestruct "HRest" as (enqIdx deqIdx) "(HIt1 & HIt2 & HAwaks & HSusps & %)".
-      apply find_index_Some in HFindIndex.
-      destruct HFindIndex as [[? [HC HPres]] HNotPres].
-      rewrite lookup_drop in HC.
-      iSplitR.
-      {
-        iPureIntro.
-        intros [_ (? & ? & HOk)].
-        replace (deqFront + S x - 1)%nat with (deqFront + x)%nat in HOk by lia.
-        by simplify_eq.
-      }
-      iExists _, _. iFrame.
-      iPureIntro.
-      repeat split; try lia.
-      assert (deqFront + x < length l)%nat; try lia.
-      apply lookup_lt_is_Some. by eauto.
-    }
-    iSplitL.
-    {
-      rewrite HCounts.
-      clear.
-      remember (count_matching _ _) as v.
-      replace (availablePermits' - S v + 1) with (availablePermits' - v) by lia.
-      done.
-    }
-    iPureIntro.
-    lia.
+    iExists _, _. iFrame. subst.
+    replace (availablePermits' - v + 1) with (availablePermits' - (v - 1)%nat) by lia.
+    iFrame "Hp". iPureIntro. lia.
   }
 
   iModIntro. wp_pures. rewrite bool_decide_decide.
@@ -400,7 +250,7 @@ Proof.
   iIntros (Φ) "!> HNoPerms HΦ".
 
   wp_lam. wp_pures. wp_bind (FAA _ _).
-  iInv "HSemInv" as (availablePermits l deqFront)
+  iInv "HSemInv" as (availablePermits v)
                       "(HPerms & >HAuth & HTq & Hp & >HPure)" "HInvClose".
   wp_faa.
   iInv "HPermInv" as (?) ">HFrag" "HPermsClose".
@@ -424,10 +274,9 @@ Proof.
     { iLeft. iFrame. eauto. }
     iMod ("HInvClose" with "[-HΦ]") as "_".
     {
-      iExists _, _, _.
+      iExists _, _.
       rewrite Nat.sub_0_r big_opL_irrelevant_element' seq_length.
-      replace (oldP + -1) with
-          (availablePermits - count_matching still_present (drop deqFront l)) by lia.
+      replace (oldP + -1) with (availablePermits - v) by lia.
       iFrame.
       iPureIntro.
       eauto.
@@ -440,23 +289,11 @@ Proof.
   rewrite Z.sub_0_l in HeqoldP.
   subst.
   iClear "HPure".
-  iAssert (⌜deqFront <= length l⌝)%I as %HDeqFront.
-  {
-    iDestruct "HTq" as "(_ & _ & _ & HRest)".
-    iDestruct "HRest" as (? ?) "(_ & _ & _ & _ & %)".
-    iPureIntro.
-    lia.
-  }
-  iMod (thread_queue_append with "[$] HTq") as "[[HIsSusp #HElExists] HTq]".
+  iMod (thread_queue_as_counter_append with "[$] HTq") as "[HIsSusp HTq]".
   iMod ("HPermsClose" with "[HFrag]") as "_"; first by eauto.
   iMod ("HInvClose" with "[-HIsSusp HNoPerms HΦ]") as "_".
   {
-    iExists _, _, _. iFrame.
-    rewrite drop_app_le.
-    2: lia.
-    rewrite count_matching_app. simpl.
-    replace (- count_matching still_present (drop deqFront l) + -1) with
-        (0%nat - (count_matching still_present (drop deqFront l) + 1)%nat) by lia.
+    iExists _, _. iFrame. replace (0%nat - S v) with (-v + - 1) by lia.
     iFrame.
     iPureIntro. lia.
   }
@@ -465,42 +302,27 @@ Proof.
 
   rewrite /is_semaphore.
 
-  awp_apply (try_enque_thread_spec (N.@"tq") with "HThreadHandle HIsSusp HNoPerms")
-            without "HΦ".
-  iInv "HSemInv" as (? l' deqFront') "(HPerms & >HAuth & HTq & Hp & >HPure)".
+  awp_apply (try_enque_thread_as_counter_spec (N.@"tq") with
+                 "HThreadHandle HIsSusp HNoPerms") without "HΦ".
+  iInv "HSemInv" as (? v') "(HPerms & >HAuth & HTq & Hp & >HPure)".
   iAaccIntro with "HTq".
   {
     iIntros "HTq !>". iSplitL; last done.
-    iExists _, _, _. iFrame.
+    iExists _, _. iFrame.
   }
-  iIntros (?) "HPures".
-  iDestruct "HPures" as "[HTq|(-> & HTq & HNoPerms & HR)]".
+  iIntros (?) "[HTq HPures]".
+  iDestruct "HPures" as "[HPures|(-> & HR & HNoPerms)]".
   2: {
     iModIntro. iSplitR "HNoPerms HR".
-    by iExists _, _, _; iFrame.
+    by iExists _, _; iFrame.
     iIntros "HΦ".
     wp_pures.
     iSpecialize ("HΦ" with "[-]").
     { iLeft. iFrame. eauto. }
     done.
   }
-  iDestruct "HTq" as (i s -> HEl) "(#HSegLoc & #HRend & HTq & HInhToken)".
-  iSplitR "HInhToken".
-  {
-    iExists _, _, _. iFrame.
-    replace (count_matching _ (drop deqFront' (alter _ _ _))) with
-      (count_matching still_present (drop deqFront' l')).
-    2: {
-      destruct (decide (i < deqFront')%nat).
-      by rewrite drop_alter //.
-      repeat rewrite count_matching_drop.
-      rewrite take_alter; try lia.
-      erewrite count_matching_alter; eauto.
-      simpl.
-      lia.
-    }
-    by iFrame.
-  }
+  iDestruct "HPures" as (i s ->) "(#HSegLoc & #HRend & HInhToken)".
+  iSplitR "HInhToken"; first by iExists _, _; iFrame.
 
   iIntros "!> HΦ". wp_pures. wp_lam. wp_pures. wp_lam. wp_pures.
   wp_apply (interruptibly_spec _ (inhabitant_token γtq i)
@@ -515,7 +337,8 @@ Proof.
       rewrite /is_thread_handle.
       iInv "HThreadHandle" as (? t) "[>% [Hℓ HThAuth]]" "HClose". simplify_eq.
       wp_load.
-      iInv "HSemInv" as (? l'' ?) "(HPerms & >HAuth & HTq & HRest)" "HClose'".
+      iInv "HSemInv" as (? ?) "(HPerms & >HAuth & HTq & HRest)" "HClose'".
+      iDestruct "HTq" as (l'' ?) "[HTq >->]".
       iAssert (▷ ⌜∃ c, l'' !! i ≡ Some (Some (cellInhabited γth _ c))⌝)%I
         as "#>HI".
       {
@@ -560,10 +383,10 @@ Proof.
         simplify_eq.
         iMod ("HClose'" with "[-Hℓ HThAuth HClose HInhTok HΦ']") as "_".
         {
-          iExists _, _, _.
-          iDestruct ("HLcRestore" with "[HArrMapsto Hℓ' HNoPerms HRend' HRest']") as "$".
-          2: by iFrame.
-          iExists _. iFrame.
+          iExists _, _.
+          iDestruct ("HLcRestore" with "[HArrMapsto Hℓ' HNoPerms HRend' HRest']") as "HLC".
+          by iExists _; iFrame.
+          iFrame. iExists _, _. by iFrame.
         }
         iMod ("HClose" with "[Hℓ HThAuth]") as "_".
         {
@@ -590,11 +413,11 @@ Proof.
         simplify_eq.
         iMod ("HClose'" with "[-Hℓ Hℓ' HThAuth HClose HHasPerm HΦ' HR]") as "_".
         {
-          iExists _, _, _.
+          iExists _, _.
           iDestruct ("HLcRestore" with "[HArrMapsto HRendHandle HIsSus HIsRes
-            HCancHandle HInhTok HResTok]") as "$".
-          2: by iFrame.
-          iExists _. iFrame. iLeft. iFrame "HInhTok". iRight. iFrame "HResTok".
+            HCancHandle HInhTok HResTok]") as "HLC".
+          { iExists _. iFrame. iLeft. iFrame "HInhTok". iRight. iFrame "HResTok". }
+          iFrame. iExists _, _. by iFrame.
         }
         iMod ("HClose" with "[Hℓ HThAuth]") as "_".
         {
@@ -617,11 +440,11 @@ Proof.
         simplify_eq.
         iMod ("HClose'" with "[-Hℓ HThAuth HClose HInhTok HΦ']") as "_".
         {
-          iExists _, _, _.
+          iExists _, _.
           iDestruct ("HLcRestore" with "[HArrMapsto HRendHandle HIsSus HIsRes
-            HCancHandle HR Hℓ' HNoPerms]") as "$".
-          2: by iFrame.
-          iExists _. iFrame. iRight. iFrame "HR Hℓ'".
+            HCancHandle HR Hℓ' HNoPerms]") as "HLC".
+          { iExists _. iFrame. iRight. iFrame "HR Hℓ'". }
+          iFrame. iExists _, _. by iFrame.
         }
         iMod ("HClose" with "[Hℓ HThAuth]") as "_".
         {
@@ -632,12 +455,12 @@ Proof.
     }
     {
       iIntros (Φ') "!> [HInhTok #HInterrupted] HΦ'". wp_pures. wp_bind (FAA _ _).
-      iClear "HElExists". move: namespaces_disjoint. clear. intros.
-      iInv "HSemInv" as (availablePermits l deqFront)
+      move: namespaces_disjoint. clear. intros.
+      iInv "HSemInv" as (availablePermits v)
                           "(HPerms & >HAuth & HTq & Hp & >HPure)" "HInvClose".
 
       remember (availablePermits - _) as oldP.
-      destruct (decide (0 <= oldP)).
+      destruct (decide (0 <= oldP)) as [HLt|HGt].
       {
         wp_faa.
         iInv "HPermInv" as (?) ">HFrag" "HPermsClose".
@@ -650,9 +473,9 @@ Proof.
           done.
         }
         iMod ("HPermsClose" with "[HFrag]") as "_"; first by eauto.
-        iAssert (⌜count_matching still_present (drop deqFront l) = 0%nat⌝)%I
-          as %HH.
+        iAssert (⌜v = 0%nat⌝)%I as %HH.
         by iDestruct "HPure" as %[HH|HH]; subst; iPureIntro; lia.
+        iDestruct "HTq" as (l deqFront) "[HTq ->]".
         iDestruct "HTq" as "(HInfArr & (HL1 & HL2 & HLAuth & HL3) & HRest)".
         iDestruct (inhabited_cell_states with "HInhTok [$]") as
             %(γt & th & [HEl|HEl]).
@@ -682,7 +505,7 @@ Proof.
           }
           iMod ("HInvClose" with "[-HΦ' HRendAbandon]") as "_".
           {
-            iExists _, _, _. iFrame "HAuth". rewrite Nat.add_1_r /=.
+            iExists _, _. iFrame "HAuth". rewrite Nat.add_1_r /=.
             iFrame "HR".
             iSplitL "HPerms".
             {
@@ -690,6 +513,11 @@ Proof.
               by repeat rewrite seq_length.
               done.
             }
+            subst.
+            rewrite Z.add_1_r Nat2Z.inj_succ Zminus_succ_l.
+            iFrame "Hp".
+            iSplitL; last by iPureIntro; right.
+            iExists _, _.
             iFrame  "HInfArr HListContents".
             rewrite alter_length.
             iDestruct "HRest" as "[HRest $]".
@@ -702,10 +530,7 @@ Proof.
               - by rewrite list_lookup_alter_ne.
             }
             rewrite drop_alter; last lia. subst.
-            rewrite HH.
-            repeat rewrite Z.sub_0_r.
-            rewrite Z.add_1_r Nat2Z.inj_succ.
-            iFrame "Hp". by iPureIntro; right.
+            by rewrite HH.
           }
           iModIntro. wp_pures. rewrite bool_decide_decide decide_True //.
           wp_pures.
@@ -715,36 +540,40 @@ Proof.
         {
           iMod ("HInvClose" with "[-HΦ']") as "_".
           {
-            iExists _, _, _.
+            iExists _, O.
             iDestruct (cell_list_contents_lookup_acc with "[$]")
                       as "[HRR HListRestore]"; first done.
-            simpl. iFrame "HInfArr HRest HAuth". subst.
+            simpl.
+            iFrame "HAuth". subst.
             rewrite HH. repeat rewrite Z.sub_0_r.
-            rewrite Z.add_1_r Nat.add_1_r /= Nat2Z.inj_succ. iFrame "Hp".
+            rewrite Z.add_1_r Nat.add_1_r /= Nat2Z.inj_succ.
+            iFrame "Hp".
             iDestruct "HRR" as (ℓ) "(HArrMapsto & HRendTh & HIsSus & HIsRes &
               HCancHandle & [[HInhTok' _]|(Hℓ & HR & [[HHasPerm HResTok]|HNoPerms])])".
             by iDestruct (inhabitant_token_exclusive with "HInhTok HInhTok'") as %[].
             {
               iDestruct ("HListRestore" with "[HArrMapsto HRendTh HIsSus HIsRes
-                HCancHandle HResTok HInhTok]") as "$".
+                HCancHandle HResTok HInhTok]") as "HLC".
               {
                 iExists _. iFrame. iLeft. iFrame.
               }
               iFrame "HR". iSplitL "HPerms".
               { iApply (big_sepL_forall' with "HPerms"); last done.
                 by repeat rewrite seq_length. }
-              iFrame. iPureIntro. right. done.
+              iSplitL; last by iPureIntro; right.
+              iExists _, _. by iFrame.
             }
             {
               iDestruct ("HListRestore" with "[HArrMapsto HRendTh HIsSus HIsRes
-                HCancHandle HInhTok HNoPerms]") as "$".
+                HCancHandle HInhTok HNoPerms]") as "HLC".
               {
                 iExists _. iFrame.
               }
               iFrame "HR". iSplitL "HPerms".
               { iApply (big_sepL_forall' with "HPerms"); last done.
                 by repeat rewrite seq_length. }
-              iFrame. iPureIntro. right. done.
+              iSplitL; last by iPureIntro; right.
+              iExists _, _. by iFrame.
             }
           }
           iModIntro. wp_pures. rewrite bool_decide_decide decide_True //.
@@ -752,44 +581,28 @@ Proof.
           iApply "HΦ'". iApply "HInterrupted".
         }
       }
-      remember (count_matching _ _) as v.
-      assert (v > 0) as HExistsNondequed by lia.
-      move: HExistsNondequed. subst. move=> HExistsNondequed.
-      apply count_matching_find_index_Some in HExistsNondequed.
-      destruct HExistsNondequed as [? HFindIndex].
 
-      iMod (do_cancel_rendezvous_spec with "HInhTok HTq") as (? ?) "HTT";
-        first done.
+      iMod (do_cancel_rendezvous_as_counter_spec with "HInhTok HTq")
+        as "[HTq HTT]"; first by lia.
 
       wp_faa.
 
-      iDestruct "HTT" as "[(HEl & HTq & HCancTok & #HRendCanc) |
-        (HEl & HTq & HLoc & HAwak & #HRendRes)]"; iDestruct "HEl" as %HEl.
+      iDestruct "HTT" as "[(HCancTok & #HRendCanc) | (HLoc & HAwak & #HRendRes)]".
       2: {
         iMod ("HInvClose" with "[-HΦ' HAwak HLoc]") as "_".
         {
-          iExists _, _, _. iFrame.
-          iSplitL "Hp".
-          2: {
-            iDestruct "HPure" as "[->|HCount]"; first by (iPureIntro; lia).
-            iDestruct "HCount" as %HCount. iPureIntro. right.
-            rewrite -drop_drop. remember (drop deqFront l) as l'.
-            replace l' with (take (S x) l' ++ drop (S x) l') in HCount;
-              last by rewrite take_drop.
-            rewrite count_matching_app in HCount. lia.
-          }
-          rewrite -drop_drop. remember (drop deqFront l) as l'.
-          rewrite count_matching_drop.
-          rewrite present_cells_in_take_Si_if_next_present_is_Si //.
-          by replace (_ - (_ - _)%nat) with
-              (availablePermits - count_matching still_present l' + 1) by lia.
+          iExists _, _. iFrame.
+          iSplitR "HPure"; last by iDestruct "HPure" as "[->|%]"; iPureIntro; lia.
+          subst.
+          by replace (availablePermits - v + 1) with (availablePermits - (v - 1)%nat) by lia.
         }
         iModIntro. wp_pures. rewrite bool_decide_decide decide_False //.
         wp_pures. wp_lam. wp_pures.
 
         awp_apply (segment_data_at_spec) without "HΦ' HLoc HAwak".
         by iPureIntro; apply Nat.mod_upper_bound; lia.
-        iInv "HSemInv" as (? ? ?) "(HHead1 & HHead2 & (HInfArr & HTail') & HTail)".
+        iInv "HSemInv" as (? ?) "(HHead1 & HHead2 & HTq & HTail)".
+        iDestruct "HTq" as (? ?) "[(HInfArr & HTail') HTail'']".
         iDestruct (is_segment_by_location with "HSegLoc HInfArr")
           as (? ?) "[HIsSeg HInfArrRestore]".
         iAaccIntro with "HIsSeg".
@@ -797,12 +610,12 @@ Proof.
           iIntros "HIsSeg".
           iDestruct ("HInfArrRestore" with "HIsSeg") as "HInfArr".
           iIntros "!>". iSplitL; last done.
-          iExists _, _, _. iFrame.
+          iExists _, _. iFrame. iExists _, _. iFrame.
         }
 
         iIntros (?) "(HIsSeg & #HArrMapsto & #HCellInv)".
         iDestruct (bi.later_wand with "HInfArrRestore HIsSeg") as "HInfArr".
-        iSplitL; first by iExists _, _, _; iFrame.
+        iSplitL; first by iExists _, _; iFrame; iExists _, _; iFrame.
         iIntros "!> (HΦ' & HLoc & HAwak)". wp_pures.
 
         iDestruct "HLoc" as (ℓ) "[#HArrMapsto' Hℓ]".
@@ -822,37 +635,10 @@ Proof.
 
       iMod ("HInvClose" with "[-HΦ' HCancTok]") as "_".
       {
-        iExists _, _, _. iFrame.
-        iSplitL "Hp".
-        2: {
-          iDestruct "HPure" as "[->|HCount]"; first by (iPureIntro; lia).
-          iDestruct "HCount" as %HCount. iPureIntro. right.
-          destruct (decide (i < deqFront)%nat).
-          - rewrite drop_alter. 2: lia.
-            rewrite -drop_drop. remember (drop deqFront l) as l'.
-            replace l' with (take (S x) l' ++ drop (S x) l') in HCount;
-              last by rewrite take_drop.
-            rewrite count_matching_app in HCount. lia.
-          - assert (deqFront <= i)%nat as HSum by lia.
-            apply nat_le_sum in HSum. destruct HSum as [? ->].
-            rewrite drop_alter'.
-            erewrite count_matching_alter; last by rewrite lookup_drop.
-            simpl. lia.
-        }
-        destruct (decide (i < deqFront)%nat).
-        - rewrite drop_alter; last lia.
-          rewrite -drop_drop. remember (drop deqFront l) as l'.
-          rewrite count_matching_drop.
-          rewrite present_cells_in_take_Si_if_next_present_is_Si //.
-          by replace (_ - (_ - _)%nat) with
-              (availablePermits - count_matching still_present l' + 1) by lia.
-        - assert (deqFront <= i)%nat as HSum by lia.
-          apply nat_le_sum in HSum. destruct HSum as [? ->].
-          rewrite drop_alter'.
-          erewrite count_matching_alter; last by rewrite lookup_drop.
-          simpl.
-          by replace (_ - (_ + _ - _)%nat) with
-              (availablePermits - count_matching still_present (drop deqFront l) + 1) by lia.
+        iExists _, _. iFrame.
+        iSplitL "Hp"; last by iDestruct "HPure" as "[->|%]"; by (iPureIntro; lia).
+        subst.
+        by replace (availablePermits - v + 1) with (availablePermits - (v - 1)%nat) by lia.
       }
 
       iModIntro. wp_pures. rewrite bool_decide_decide decide_False //. wp_pures.
@@ -860,7 +646,8 @@ Proof.
 
       awp_apply (segment_data_at_spec) without "HΦ' HCancTok".
       by iPureIntro; apply Nat.mod_upper_bound; lia.
-      iInv "HSemInv" as (? ? ?) "(HHead1 & HHead2 & (HInfArr & HTail') & HTail)".
+      iInv "HSemInv" as (? ?) "(HHead1 & HHead2 & HTq & HTail)".
+      iDestruct "HTq" as (? ?) "[(HInfArr & HTail') HTail'']".
       iDestruct (is_segment_by_location with "HSegLoc HInfArr")
         as (? ?) "[HIsSeg HInfArrRestore]".
       iAaccIntro with "HIsSeg".
@@ -868,17 +655,18 @@ Proof.
         iIntros "HIsSeg".
         iDestruct ("HInfArrRestore" with "HIsSeg") as "HInfArr".
         iIntros "!>". iSplitL; last done.
-        iExists _, _, _. iFrame.
+        iExists _, _; iFrame.
+        iExists _, _; iFrame.
       }
       iIntros (ℓ) "(HIsSeg & #HArrMapsto & #HCellInv)".
       iDestruct (bi.later_wand with "HInfArrRestore HIsSeg") as "HInfArr".
-      iSplitL; first by iExists _, _, _; iFrame.
+      iSplitL; first by iExists _, _; iFrame; iExists _, _; iFrame.
       iIntros "!> (HΦ' & HCancTok)". wp_pures.
 
       awp_apply getAndSet.getAndSet_spec without "HΦ'".
       move: namespaces_disjoint. clear. intros.
-      iInv "HSemInv" as (? l ?) "(HHead1 & HHead2 &
-        (HInfArr & HListContents & HTail') & HTail)".
+      iInv "HSemInv" as (? ?) "(HHead1 & HHead2 & HTq & HTail)".
+      iDestruct "HTq" as (l ?) "[(HInfArr & HListContents & HTail') >->]".
       iAssert (▷ ⌜∃ γt th, l !! i = Some (Some (cellInhabited γt th
                                   (Some cellCancelled)))⌝)%I
               as "#>HEl".
@@ -919,8 +707,8 @@ Proof.
         iAaccIntro with "HAacc".
         {
           iIntros "[Hℓ _]". iFrame "HCancTok".
-          iIntros "!>". iExists _, _, _.
-          iFrame.
+          iIntros "!>". iExists _, _. iFrame. iExists _, _. iFrame.
+          iSplitL; last by iPureIntro.
           iApply "HListContentsRestore".
           iExists _. iFrame "HArrMapsto' HRendHandle HIsSus HInhTok".
           iRight. iLeft. iFrame. iRight. iFrame.
@@ -929,7 +717,9 @@ Proof.
         iIntros "Hℓ !>".
         iSplitR "HAwak".
         {
-          iExists _, _, _. iFrame.
+          iExists _, _. iFrame.
+          iExists _, _. iFrame.
+          iSplitL; last by iPureIntro.
           iApply "HListContentsRestore".
           iExists _. iFrame "HArrMapsto' HRendHandle HIsSus HInhTok".
           iRight. iRight. iFrame. iLeft. iFrame.
@@ -943,8 +733,8 @@ Proof.
       iAaccIntro with "HAacc".
       {
         iIntros "[Hℓ _]". iFrame "HCancTok".
-        iIntros "!>". iExists _, _, _.
-        iFrame.
+        iIntros "!>". iExists _, _. iFrame. iExists _, _. iFrame.
+        iSplitL; last by iPureIntro.
         iApply "HListContentsRestore".
         iExists _. iFrame "HArrMapsto' HRendHandle HIsSus HInhTok".
         iLeft. iFrame.
@@ -953,7 +743,8 @@ Proof.
       iIntros "Hℓ !>".
       iSplitR "HCancHandle".
       {
-        iExists _, _, _. iFrame.
+        iExists _, _. iFrame. iExists _, _. iFrame.
+        iSplitL; last by iPureIntro.
         iApply "HListContentsRestore".
         iExists _. iFrame "HArrMapsto' HRendHandle HIsSus HInhTok".
         iRight. iRight. iFrame. iRight. iFrame.
@@ -963,13 +754,14 @@ Proof.
       awp_apply (segment_cancel_cell_spec with "HSegLoc HCancHandle") without "HΦ'".
       by apply Nat.mod_upper_bound; lia.
 
-      iInv "HSemInv" as (? ? ?) "(HHead1 & HHead2 & (HInfArr & HTail') & HTail)".
+      iInv "HSemInv" as (? ?) "(HHead1 & HHead2 & HTq & HTail)".
+      iDestruct "HTq" as (? ?) "[(HInfArr & HTail') HPf]".
       iAaccIntro with "HInfArr".
       {
-        iIntros "$ !>". iExists _, _, _. iFrame.
+        iIntros "$ !>". iExists _, _. iFrame. iExists _, _. iFrame.
       }
       iIntros (?) "$ !>". iSplitL.
-      by iExists _, _, _; iFrame.
+      by iExists _, _; iFrame; iExists _, _; iFrame.
       iIntros "HΦ". wp_pures. iApply "HΦ". iAssumption.
     }
   }
