formal-proofs/theories/lib/barrier/barrier.v
@@ -1,0 +1,115 @@
+From iris.heap_lang Require Import notation.
+
+Require Import SegmentQueue.lib.thread_queue.thread_queue.
+
+Section impl.
+
+Variable segment_size : positive.
+Variable limit: positive.
+
+Definition new_barrier : val :=
+  λ: <>, (ref #0, new_thread_queue segment_size #()).
+
+Definition forRange : val :=
+  rec: "loop" "n" "fn" :=
+    if: "n" ≤ #0
+    then #()
+    else "loop" ("n"-#1) "fn" ;; "fn" ("n"-#1).
+
+Definition cancellation_handler : val :=
+  rec: "loop" "ctr" "head" "deqIdx" "canceller" <>:=
+  let: "arrived" := ! "ctr"
+  in if: #(Pos.to_nat limit) ≤ "arrived"
+     then #false
+     else
+       if: CAS "ctr" "arrived" ("arrived" + #1)
+       then if: "canceller" #()
+            then #()
+            else resume segment_size "head" "deqIdx"
+              ;;
+            #true
+       else "loop" "ctr" "head" "deqIdx" "canceller".
+
+Definition await : val :=
+  λ: "threadHandle" "ctr" "tail" "enqIdx" "head" "deqIdx",
+  let: "p" := FAA "ctr" #1
+  in if: "p" = #(Pos.to_nat limit-1)
+     then forRange "p" (λ: "i", resume segment_size "head" "deqIdx")
+     else suspend segment_size (cancellation_handler "ctr" "head" "deqIdx")
+                  "cancHandle" "threadHandle" "tail" "enqIdx".
+
+End impl.
+
+From iris.base_logic.lib Require Import invariants.
+From iris.heap_lang Require Import proofmode.
+From iris.algebra Require Import auth.
+From iris.algebra Require Import list gset excl csum.
+From iris.program_logic Require Import atomic.
+
+Require Import SegmentQueue.lib.infinite_array.infinite_array_impl.
+Require Import SegmentQueue.lib.infinite_array.iterator.
+Require Import SegmentQueue.lib.util.interruptibly.
+
+Section proof.
+
+Context `{!heapG Σ}.
+
+Theorem forRange_spec (Φ: nat -> iProp Σ) (e: val):
+  (∀ i, {{{ Φ i }}}
+           e #i
+         {{{ v, RET v; Φ (S i) }}})
+   -∗
+   (∀ n, {{{ Φ O }}}
+           forRange #n e
+         {{{ v, RET v; Φ n }}}).
+Proof.
+  iIntros "#HE" (n Ψ).
+  iInduction n as [|n'] "IH" forall (Ψ); iIntros "!> HΦ0 HΨ"; wp_lam; wp_pures.
+  by iApply "HΨ".
+  replace #(S n' - 1) with #n'; last by congr (fun x => LitV (LitInt x)); lia.
+  wp_bind (forRange _ _).
+  wp_apply ("IH" with "HΦ0").
+  iIntros (v) "HΦn".
+  wp_pures.
+  replace #(S n' - 1) with #n'; last by congr (fun x => LitV (LitInt x)); lia.
+  by wp_apply ("HE" with "HΦn").
+Qed.
+
+End proof.
+
+Section barrier_proof.
+
+Variable (limit: positive).
+
+Notation algebra := (authR (optionUR (csumR positiveR positiveR))).
+
+Class barrierG Σ := BarrierG { barrier_inG :> inG Σ algebra }.
+Definition barrierΣ : gFunctors := #[GFunctor algebra].
+Instance subG_barrierΣ {Σ} : subG barrierΣ Σ -> barrierG Σ.
+Proof. solve_inG. Qed.
+
+Context `{iArrayG Σ} `{iteratorG Σ} `{heapG Σ} `{threadQueueG Σ} `{barrierG Σ}
+        `{parkingG Σ} `{interruptiblyG Σ}.
+Variable (Nth: namespace) (N: namespace).
+Variable (namespaces_disjoint : Nth ## N).
+Notation iProp := (iProp Σ).
+
+Variable (segment_size: positive).
+
+Definition barrier_entry_piece γ := own γ (◯ (Some (Cinl 1%positive))).
+Definition barrier_exit_piece γ := own γ (◯ (Some (Cinr 1%positive))).
+
+Definition is_barrier_inv γ (ℓ: loc) (n: nat)
+  (epℓ eℓ dpℓ dℓ: loc) (γa γtq γe γd: gname) :=
+  (∃ l deqFront, own γ (● (Some (Cinl limit))) ∗
+    ℓ ↦ #n ∗ (if decide (n < Pos.to_nat limit)%nat
+              then [∗] replicate n (barrier_entry_piece γ)
+              else True) ∗
+    is_thread_queue (N .@ "tq") Nth segment_size True (barrier_exit_piece γ)
+    γa γtq γe γd eℓ epℓ dℓ dpℓ l deqFront ∗
+    let v := count_matching still_present (drop deqFront l) in
+    (⌜if decide (n < Pos.to_nat limit)%nat then v = n else v = O⌝))%I.
+
+
+
+End barrier_proof.
