formal-proofs/theories/lib/thread_queue/thread_queue_as_counter.v
@@ -1,0 +1,289 @@
+From iris.heap_lang Require Import notation.
+From iris.base_logic.lib Require Import invariants.
+From iris.heap_lang Require Import proofmode.
+From iris.algebra Require Import auth.
+From iris.algebra Require Import list gset excl csum.
+From iris.program_logic Require Import atomic.
+Require Import SegmentQueue.lib.thread_queue.thread_queue.
+Require Import SegmentQueue.lib.infinite_array.infinite_array_impl.
+Require Import SegmentQueue.lib.infinite_array.iterator.
+Require Import SegmentQueue.lib.util.interruptibly.
+
+Section proof.
+
+Context `{iArrayG Σ} `{iteratorG Σ} `{heapG Σ} `{threadQueueG Σ}
+        `{parkingG Σ} `{interruptiblyG Σ}.
+
+Variable (N Nth: namespace).
+Variable (segment_size: positive).
+
+Definition thread_queue_as_counter E R γa γtq γe γd eℓ epℓ dℓ dpℓ n :=
+  (∃ l deqFront,
+    is_thread_queue N Nth segment_size E R γa γtq γe γd eℓ epℓ dℓ dpℓ l deqFront ∗
+                    ⌜n = count_matching still_present (drop deqFront l)⌝)%I.
+
+Lemma try_deque_thread_as_counter_spec E R γa γtq γe γd (eℓ epℓ dℓ dpℓ: loc):
+  ▷ awakening_permit γtq
+    -∗
+  <<< ∀ (n: nat), ▷ thread_queue_as_counter E R γa γtq γe γd eℓ epℓ dℓ dpℓ n >>>
+    ((try_deque_thread segment_size) #dpℓ) #dℓ @ ⊤ ∖ ↑N
+  <<< ∃ v : val, ▷ E ∗ ▷ thread_queue_as_counter E R γa γtq γe γd eℓ epℓ dℓ dpℓ n ∗
+                   (⌜v = #()⌝ ∨
+                    (∃ i γt (th: loc),
+                        ⌜v = #th⌝ ∧ ▷ rendezvous_thread_handle Nth γtq γt th i ∗
+                                      (resumer_token γtq i ∗ rendezvous_resumed γtq i ∨
+                                       thread_doesnt_have_permits γt)
+                   )), RET v >>>.
+Proof.
+  iIntros "HAwak" (HΦ) "AU".
+  awp_apply (try_deque_thread_spec with "HAwak").
+  iApply (aacc_aupd_commit with "AU"); first done.
+  iIntros (n) "HTq".
+  iDestruct "HTq" as (l deqFront) "[HTq >->]".
+  iAaccIntro with "HTq".
+  {
+    iIntros "HTq !>". iSplitL; first by iExists _, _; iFrame.
+    iIntros "$ //".
+  }
+  iIntros (v) "[$ HState]". iExists _; iSplitL; last by iIntros "!> $".
+  iDestruct "HState" as (i) "[HState|HState]".
+  - iDestruct "HState" as "[(HEl & -> & HTq) HRend]".
+    iDestruct "HEl" as %HEl.
+    iSplitL "HTq"; last by iLeft.
+    destruct (decide (i < deqFront)%nat).
+    2: {
+      iDestruct "HTq" as "(_ & (_ & >HResumerStage & _) & _)".
+      rewrite big_sepL_forall.
+      iSpecialize ("HResumerStage" $! (i - deqFront)%nat _ with "[]").
+      {
+        iPureIntro.
+        rewrite lookup_drop.
+        replace (deqFront + (i - deqFront))%nat with i by lia.
+        rewrite list_lookup_alter.
+        rewrite HEl. done.
+      }
+      simpl.
+      iDestruct "HResumerStage" as %HContra.
+      discriminate.
+    }
+    iExists _, deqFront.
+    iFrame.
+    iPureIntro.
+    by rewrite drop_alter.
+  - iDestruct "HState" as (γt th) "[#HThreadHandle [HState|HState]]".
+    2: {
+      iDestruct "HState" as "[HState (-> & HTq & HNoPerms)]".
+      iSplitL "HTq"; first by iExists _, _; iFrame.
+      iRight. iExists _, _, _. iSplitR; first by iPureIntro.
+      iFrame "HThreadHandle". by iRight.
+    }
+    iDestruct "HState" as (HEl ->) "(HTq & #HRendRes & HResTok)".
+    {
+      destruct (decide (i < deqFront)%nat).
+      2: {
+        iDestruct "HTq" as "(_ & (_ & >HResumerStage & _) & _)".
+        rewrite big_sepL_forall.
+        iSpecialize ("HResumerStage" $! (i - deqFront)%nat _ with "[]").
+        {
+          iPureIntro.
+          rewrite lookup_drop.
+          replace (deqFront + (i - deqFront))%nat with i by lia.
+          rewrite list_lookup_alter.
+          rewrite HEl. done.
+        }
+        simpl.
+        iDestruct "HResumerStage" as %HContra.
+
+        discriminate.
+      }
+      iSplitL "HTq".
+      { iExists _, _. iFrame. iPureIntro. by rewrite drop_alter. }
+      iRight. iExists _, _, _. iSplitR; first by iPureIntro.
+      iFrame "HThreadHandle".
+      by iLeft; iFrame.
+    }
+Qed.
+
+Lemma try_enque_thread_as_counter_spec E R γa γtq γe γd γt (eℓ epℓ dℓ dpℓ th : loc):
+  is_thread_handle Nth γt #th -∗
+  suspension_permit γtq -∗ thread_doesnt_have_permits γt -∗
+  <<< ∀ (n: nat), ▷ thread_queue_as_counter E R γa γtq γe γd eℓ epℓ dℓ dpℓ n >>>
+    (((try_enque_thread segment_size) #th) #epℓ) #eℓ @ ⊤ ∖ ↑N
+  <<< ∃ v, ▷ thread_queue_as_counter E R γa γtq γe γd eℓ epℓ dℓ dpℓ n ∗
+           ((∃ (i: nat) (s: loc),
+             ⌜v = InjRV (#s, #(i `mod` Pos.to_nat segment_size)%nat)⌝ ∧
+             segment_location γa (i `div` Pos.to_nat segment_size) s ∗
+             rendezvous_thread_handle Nth γtq γt th i ∗ inhabitant_token γtq i
+            ) ∨
+            (⌜v = InjLV #()⌝ ∧ ▷ R ∗ thread_doesnt_have_permits γt)),
+  RET v >>>.
+Proof.
+  iIntros "HTh HIsSus HNoPerms" (Φ) "AU".
+  awp_apply (try_enque_thread_spec with "HTh HIsSus HNoPerms").
+  iApply (aacc_aupd_commit with "AU"); first done.
+  iIntros (n) "HTq".
+  iDestruct "HTq" as (l deqFront) "[HTq >->]".
+  iAaccIntro with "HTq".
+  {
+    iIntros "HTq !>". iSplitL; first by iExists _, _; iFrame.
+    iIntros "$ //".
+  }
+  iIntros (v) "HPures".
+  iExists v. iSplitL; last by iIntros "!> $".
+  iDestruct "HPures" as "[HTq|(-> & HTq & HNoPerms & HR)]".
+  2: {
+    iSplitL "HTq". iExists _, _; by iFrame "HTq".
+    iRight. by iFrame.
+  }
+  iDestruct "HTq" as (i s -> HEl) "(#HSegLoc & #HRend & HTq & HInhToken)".
+  iSplitL "HTq"; last by iLeft; iExists i, s; iSplitR;
+    [iPureIntro|iFrame "HSegLoc HRend HInhToken"].
+  iExists _, _. iFrame.
+  iPureIntro.
+  destruct (decide (i < deqFront)%nat).
+  by rewrite drop_alter //.
+  repeat rewrite count_matching_drop.
+  rewrite take_alter; try lia.
+  erewrite count_matching_alter; eauto.
+  simpl.
+  lia.
+Qed.
+
+Lemma thread_queue_as_counter_append E R γa γtq γe γd (eℓ epℓ dℓ dpℓ : loc) n:
+  E -∗ thread_queue_as_counter E R γa γtq γe γd eℓ epℓ dℓ dpℓ n
+    ==∗ suspension_permit γtq ∗
+    thread_queue_as_counter E R γa γtq γe γd eℓ epℓ dℓ dpℓ (S n).
+Proof.
+  iIntros "HE HTq".
+  iDestruct "HTq" as (l deqFront) "[HTq ->]".
+  iAssert (⌜(deqFront <= length l)%nat⌝)%I as %HDeqFront.
+  {
+    iDestruct "HTq" as "(_ & _ & _ & HRest)".
+    iDestruct "HRest" as (? ?) "(_ & _ & _ & _ & %)".
+    iPureIntro.
+    lia.
+  }
+  iMod (thread_queue_append with "HE HTq") as "[[$ _] HTq]".
+  iExists _, _. iFrame. iPureIntro.
+  rewrite drop_app_le // count_matching_app /=. lia.
+Qed.
+
+Lemma thread_queue_as_counter_unpark_spec E R γa γtq γe γd γt (eℓ epℓ dℓ dpℓ: loc) (th: loc) i:
+  rendezvous_resumed γtq i -∗
+  is_thread_handle Nth γt #th -∗
+  rendezvous_thread_locs_state γtq γt th i -∗
+  <<< ∀ n, resumer_token γtq i ∗ ▷ thread_queue_as_counter E R γa γtq γe γd eℓ epℓ dℓ dpℓ n >>>
+    unpark #th @ ⊤ ∖ ↑Nth
+  <<< ▷ thread_queue_as_counter E R γa γtq γe γd eℓ epℓ dℓ dpℓ n, RET #() >>>.
+Proof.
+  iIntros "HRendRes HIsThread HThreadLocs" (Φ) "AU".
+  awp_apply (thread_queue_unpark_spec with "HRendRes HIsThread HThreadLocs").
+  iApply (aacc_aupd_commit with  "AU"); first done.
+  iIntros (n) "[HResTok HTq]". iDestruct "HTq" as (? ?) "[HTq >->]".
+  iCombine "HResTok" "HTq" as "HAacc".
+  iAaccIntro with "HAacc".
+  {
+    iIntros "[$ HTq]". iSplitL; last by iIntros "!> $".
+    iExists _, _. by iFrame.
+  }
+  iIntros "HTq".
+  iSplitL; last by iIntros "!> $".
+  iExists _, _. by iFrame.
+Qed.
+
+Theorem count_matching_find_index_Some A (P: A -> Prop) (H': forall x, Decision (P x)) l:
+  (count_matching P l > 0)%nat -> is_Some (find_index P l).
+Proof.
+  induction l; simpl; first lia.
+  destruct (decide (P a)); first by eauto.
+  destruct (find_index P l); by eauto.
+Qed.
+
+Lemma thread_as_counter_register_for_dequeue E R γa γtq γe γd (eℓ epℓ dℓ dpℓ : loc) n:
+  (n > 0)%nat ->
+  R -∗ thread_queue_as_counter E R γa γtq γe γd eℓ epℓ dℓ dpℓ n
+    ==∗ awakening_permit γtq ∗
+        thread_queue_as_counter E R γa γtq γe γd eℓ epℓ dℓ dpℓ (n - 1).
+Proof.
+  iIntros (HNPos) "HR HTq".
+  iDestruct "HTq" as (l deqFront) "[HTq ->]".
+
+  apply count_matching_find_index_Some in HNPos.
+  destruct HNPos as [? HFindIndex].
+
+  iDestruct "HTq" as "(HInfArr & HListContents & % & HRest)".
+  iDestruct (cell_list_contents_register_for_dequeue
+               with "HR HListContents") as ">[[$ #HDeqFront] [HListContents HCounts]]".
+  by eauto.
+
+  iExists _, _. iFrame "HListContents". iFrame.
+  iSplitL "HRest".
+  {
+    iDestruct "HRest" as (enqIdx deqIdx) "(HIt1 & HIt2 & HAwaks & HSusps & %)".
+    apply find_index_Some in HFindIndex.
+    destruct HFindIndex as [[? [HC HPres]] HNotPres].
+    rewrite lookup_drop in HC.
+    iSplitR.
+    {
+      iPureIntro.
+      intros [_ (? & ? & HOk)].
+      replace (deqFront + S x - 1)%nat with (deqFront + x)%nat in HOk by lia.
+      by simplify_eq.
+    }
+    iExists _, _. iFrame.
+    iPureIntro.
+    repeat split; try lia.
+    assert (deqFront + x < length l)%nat; try lia.
+    apply lookup_lt_is_Some. by eauto.
+  }
+  iDestruct "HCounts" as %HCounts.
+  iPureIntro.
+  rewrite HCounts. lia.
+Qed.
+
+Lemma do_cancel_rendezvous_as_counter_spec E R γa γtq γe γd (eℓ epℓ dℓ dpℓ : loc) (n i : nat):
+  (n > 0)%nat ->
+  inhabitant_token γtq i -∗
+  ▷ thread_queue_as_counter E R γa γtq γe γd eℓ epℓ dℓ dpℓ n ==∗
+  ▷ (thread_queue_as_counter E R γa γtq γe γd eℓ epℓ dℓ dpℓ (n - 1)%nat ∗
+      (canceller_token γtq i ∗ rendezvous_cancelled γtq i
+        ∨ (∃ ℓ : loc, array_mapsto segment_size γa i ℓ ∗ ▷ ℓ ↦ InjRV #0)
+              ∗ awakening_permit γtq ∗ rendezvous_resumed γtq i)).
+Proof.
+  iIntros (HNGt) "HInhToken HTq".
+  iDestruct "HTq" as (l deqFront) "[HTq >->]".
+  apply count_matching_find_index_Some in HNGt.
+  destruct HNGt as [? HFindIndex].
+
+  iMod (do_cancel_rendezvous_spec with "HInhToken HTq") as (? ?) "HTT";
+    first done.
+
+  iDestruct "HTT" as "[(>HEl & HTq & HCancTok & #HRendCanc) |
+    (>HEl & HTq & HLoc & HAwak & #HRendRes)]"; iDestruct "HEl" as %HEl.
+  2: {
+    iSplitR "HLoc HAwak"; last by iRight; iFrame.
+    iExists _, _. iFrame.
+    rewrite -drop_drop. remember (drop _ _) as l'.
+    iPureIntro.
+    rewrite count_matching_drop.
+    by rewrite present_cells_in_take_Si_if_next_present_is_Si.
+  }
+
+  iSplitR "HCancTok"; last by iLeft; iFrame.
+  iExists _, _. iFrame.
+  iPureIntro.
+
+  destruct (decide (i < deqFront)%nat) as [HLt|HGt].
+  - rewrite drop_alter; last lia.
+    rewrite -drop_drop. remember (drop deqFront l) as l'.
+    rewrite count_matching_drop.
+    rewrite present_cells_in_take_Si_if_next_present_is_Si //.
+  - assert (deqFront <= i)%nat as HSum by lia.
+    apply nat_le_sum in HSum. destruct HSum as [? ->].
+    rewrite drop_alter'.
+    erewrite count_matching_alter; last by rewrite lookup_drop.
+    simpl.
+    lia.
+Qed.
+
+End proof.
